fix Division; without proving memory safety

code/experimental/rsa/Division.fst
@@ -4,70 +4,43 @@ open FStar.HyperStack.All
 open FStar.Buffer
 open FStar.Int.Cast
 
-open Convert
-open Shift
+open Shift 
 open Comparison
 open Addition
 
-module ST = FStar.HyperStack.ST
 module U32 = FStar.UInt32
 module U64 = FStar.UInt64
 
 type bignum = buffer FStar.UInt64.t
-
 type lbignum (len:U32.t) = 
      b:bignum{length b = U32.v len} 
 
 type bnlen = (l:U32.t{U32.v l > 0 /\ U32.v l <= 8192})
-type rem_state (rLen:bnlen) (modLen:bnlen) = lbignum U32.(rLen +^ rLen +^ modLen +^ modLen)
 
-let get_r_i #r #m (st:rem_state r m) : lbignum r = Buffer.sub st 0ul r
-let get_tmp #r #m (st:rem_state r m) : lbignum r = Buffer.sub st r r
-let get_mod #r #m (st:rem_state r m) : lbignum m = Buffer.sub st U32.(r +^ r) m
-let get_mod_1 #r #m (st:rem_state r m) :lbignum m = Buffer.sub st U32.(r +^ r +^ m) m
-
-let rem_state_inv r m (st:rem_state r m) = 
-           let r_i = get_r_i st in
-           let tmp = get_tmp st in
-           let mod = get_mod st in
-           let mod_1 = get_mod_1 st in
-           let r = frameOf r_i in
-	     r == frameOf mod /\
-	     r == frameOf mod_1 /\
-	     r == frameOf tmp /\
-	     disjoint r_i tmp /\
-	     disjoint r_i mod /\
-	     disjoint r_i mod_1 /\ 
-	     disjoint tmp mod /\ 
-	     disjoint tmp mod_1 /\ 
-       	     disjoint mod mod_1 
-
-
-let rem_state_st_inv (rLen:bnlen) (modLen:bnlen) (st:rem_state rLen modLen) (h:FStar.HyperStack.mem) = 
-	     rem_state_inv rLen modLen st /\ live h st
-		       
 val remainder_loop:
-    rLen:bnlen -> modLen:bnlen{ U32.v modLen = U32.v rLen} ->
-    count:U32.t ->  st:rem_state rLen modLen -> Stack unit
-    (requires (fun h -> rem_state_st_inv rLen modLen st h))
-    (ensures (fun h0 _ h1 -> rem_state_st_inv rLen modLen st h1 /\ 
-			   modifies_1 st h0 h1))
+    rLen:bnlen ->
+    modLen:bnlen ->
+    r_i:lbignum rLen ->
+    mod:lbignum modLen ->
+    count:U32.t -> Stack unit
+        (requires (fun h -> live h r_i /\ live h mod))
+	    (ensures (fun h0 _ h1 -> live h0 r_i /\ live h0 mod /\
+            live h1 r_i /\ live h1 mod /\ modifies_2 mod r_i h0 h1))
 
-#set-options "--z3rlimit 300 --max_fuel 0"
-let rec remainder_loop rLen modLen count st =
-  if U32.(count >^ 0ul) then begin
-    let tmp = get_tmp st in
-    let mod_1 = get_mod_1 st in
-    let r_i = get_r_i st in
-    let mod = get_mod st in
-    rshift1 modLen mod mod_1;
-    let tmp_b = isMore modLen rLen mod r_i in
-    (if not tmp_b then
-        (sub rLen modLen r_i mod tmp;
-        blit tmp 0ul r_i 0ul rLen));
-    blit mod_1 0ul mod 0ul modLen;
-    remainder_loop rLen modLen U32.(count -^ 1ul) st 
-    end
+let rec remainder_loop rLen modLen r_i mod count =
+    push_frame();
+    let mod1 = create 0uL modLen in
+    let tmp = create 0uL rLen in
+    (if U32.(count >^ 0ul) then begin
+        rshift1 modLen mod mod1;
+        let tmp_b = isMore modLen rLen mod r_i in
+        (if not tmp_b then begin
+		    sub rLen modLen r_i mod tmp; 
+            blit tmp 0ul r_i 0ul rLen end);
+        blit mod1 0ul mod 0ul modLen;    
+        remainder_loop rLen modLen r_i mod U32.(count -^ 1ul)
+        end);
+    pop_frame()
 
 (* res = a % mod *)
 val remainder:
@@ -75,28 +48,22 @@ val remainder:
     modLen:bnlen{U32.v modLen <= U32.v aLen} ->
     resLen:bnlen{U32.v resLen <= U32.v modLen} ->
     diffBits:U32.t{U32.v diffBits = op_Multiply 64 (U32.v aLen - U32.v modLen)} ->
-    a:lbignum aLen -> mod:lbignum modLen{disjoint a mod} ->
-    res:lbignum resLen{disjoint a res /\ disjoint mod res} -> Stack unit
-	(requires (fun h -> live h a /\ live h mod /\ live h res))
-	(ensures (fun h0 _ h1 -> live h0 a /\ live h0 mod /\  live h0 res /\
-        live h1 a /\ live h1 mod /\ live h1 res /\ modifies_1 res h0 h1))
-
-#set-options "--z3rlimit 150"
+    a:lbignum aLen ->
+    mod:lbignum modLen ->
+    res:lbignum resLen -> Stack unit
+	    (requires (fun h -> live h a /\ live h mod /\ live h res))
+	    (ensures (fun h0 _ h1 -> live h0 a /\ live h0 mod /\  live h0 res /\
+            live h1 a /\ live h1 mod /\ live h1 res /\ modifies_1 res h0 h1))
 
 let remainder aLen modLen resLen diffBits a mod res =
     push_frame();
     let modk = U32.(diffBits /^ 64ul) in
     let mod1Len = U32.(modLen +^ modk +^ 1ul) in
-    assume(U32.v mod1Len > 0 /\ U32.v mod1Len <= 8192);
-    let a1Len = U32.(aLen +^ 1ul) in
-    assume(U32.v a1Len > 0 /\ U32.v a1Len <= 8192);
-    let mod1Len: bnlen = mod1Len in
-    let a1Len: bnlen = a1Len in
-    let st : rem_state a1Len mod1Len = create 0uL U32.(a1Len +^ a1Len +^ mod1Len +^ mod1Len) in
-    let mod1 = get_mod_1 st in
-    let r_0 = get_r_i st in
+    let mod1 = create 0uL mod1Len in
     lshift modLen mod diffBits mod1;
-    blit a 0ul r_0 1ul aLen;
-    remainder_loop a1Len mod1Len diffBits st;
-    blit r_0 0ul res 0ul resLen;
+    let a1Len = U32.(aLen +^ 1ul) in
+    let r0 = create 0uL a1Len in
+    blit a 0ul r0 0ul aLen;
+    remainder_loop a1Len mod1Len r0 mod1 diffBits;
+    blit r0 0ul res 0ul resLen;
     pop_frame()
